feat(Time_Refinement) adapt Time Refinement

thys/nrest/Time_Refinement.thy
@@ -1,36 +1,47 @@
 theory Time_Refinement
-imports NREST
+imports NREST NREST_Type_Classes
 begin
 
 
 
 
-section "time refine"
+section "time refine" 
 
-
-definition timerefine ::"('b \<Rightarrow> 'c \<Rightarrow> enat)  \<Rightarrow> ('a, 'b \<Rightarrow> enat) nrest \<Rightarrow> ('a, 'c \<Rightarrow> enat) nrest"  where
-  "timerefine R m = (case m of FAILi \<Rightarrow> FAILi |
+(* mult_zero for wfR_finite_mult_left *)
+definition timerefine ::"('b \<Rightarrow> ('c,'d::{complete_lattice,comm_monoid_add,times,mult_zero}) acost)
+                             \<Rightarrow> ('a, ('b,'d) acost) nrest \<Rightarrow> ('a, ('c,'d) acost) nrest"
+  where "timerefine R m = (case m of FAILi \<Rightarrow> FAILi |
                 REST M \<Rightarrow> REST (\<lambda>r. case M r of None \<Rightarrow> None |
-                  Some cm \<Rightarrow> Some (\<lambda>cc. Sum_any (\<lambda>ac. cm ac * R ac cc))))"
+                  Some cm \<Rightarrow> Some (acostC (\<lambda>cc. Sum_any (\<lambda>ac. the_acost cm ac * the_acost (R ac) cc)))))"
 
-definition wfn :: "('a, 'b \<Rightarrow> enat) nrest \<Rightarrow> bool" where
+
+definition timerefineF ::"('b \<Rightarrow> ('c,'d::{complete_lattice,comm_monoid_add,times,mult_zero}) acost)
+                             \<Rightarrow> ('a \<Rightarrow> ('b,'d) acost option) \<Rightarrow> ('a \<Rightarrow> ('c,'d) acost option)"
+  where "timerefineF R M = (\<lambda>r. case M r of None \<Rightarrow> None |
+                  Some cm \<Rightarrow> Some (acostC (\<lambda>cc. Sum_any (\<lambda>ac. the_acost cm ac * the_acost (R ac) cc))))"
+
+lemma timerefine_alt: "timerefine R m = case_nrest FAILi (\<lambda>M. SPECT (timerefineF R M)) m"
+  unfolding timerefine_def timerefineF_def ..
+
+lemma timerefine_SPECT: "timerefine R (SPECT Q) = SPECT (timerefineF R Q)" 
+  unfolding timerefine_alt by simp
+
+
+definition wfn :: "('a, ('c,'d::{complete_lattice,comm_monoid_add,times,mult_zero}) acost) nrest \<Rightarrow> bool" where
   "wfn m = (case m of FAILi \<Rightarrow> True |
-                REST M \<Rightarrow> \<forall>r\<in>dom M. (case M r of None \<Rightarrow> True | Some cm \<Rightarrow> finite {x. cm x \<noteq> 0}))"
+                REST M \<Rightarrow> \<forall>r\<in>dom M. (case M r of None \<Rightarrow> True | Some cm \<Rightarrow> finite {x. the_acost cm x \<noteq> 0}))"
 
-definition wfR :: "('b \<Rightarrow> 'c \<Rightarrow> enat) \<Rightarrow> bool" where
-  "wfR R = (finite {(s,f). R s f \<noteq> 0})"
-
-
+definition wfR :: "('b \<Rightarrow> ('c, _::mult_zero) acost) \<Rightarrow> bool" where
+  "wfR R = (finite {(s,f). the_acost (R s) f \<noteq> 0})"
 
 
-
-lemma wfR_fst: "\<And>y. wfR R \<Longrightarrow> finite {x. R x y \<noteq> 0}"
-  unfolding wfR_def apply(rule finite_subset[where B="fst ` {(s, f). R s f \<noteq> 0}"])
+lemma wfR_fst: "\<And>y. wfR R \<Longrightarrow> finite {x. the_acost (R x) y \<noteq> 0}"
+  unfolding wfR_def apply(rule finite_subset[where B="fst ` {(s, f). the_acost (R s) f \<noteq> 0}"])
   subgoal by auto
   apply(rule finite_imageI) by simp
 
-lemma wfR_snd: "\<And>x. wfR R \<Longrightarrow> finite {y. R x y \<noteq> 0}"
-  unfolding wfR_def apply(rule finite_subset[where B="snd ` {(s, f). R s f \<noteq> 0}"])
+lemma wfR_snd: "\<And>s. wfR R \<Longrightarrow> finite {y. the_acost (R s) y \<noteq> 0}"
+  unfolding wfR_def apply(rule finite_subset[where B="snd ` {(s, f). the_acost (R s) f \<noteq> 0}"])
   subgoal by auto
   apply(rule finite_imageI) by simp
 
@@ -41,30 +52,30 @@ lemma finite_same_support:
 
 lemma 
   finite_wfR_middle_mult:
+  fixes R1 :: "_ \<Rightarrow> ('a, 'b::{semiring_no_zero_divisors}) acost"
   assumes "wfR R1" "wfR R2"
-  shows "finite {a. R2 x a * R1 a y \<noteq> (0::enat)}"
+  shows "finite {a. the_acost (R2 x) a * the_acost (R1 a) y \<noteq> 0}"
 proof -
-  have "{a. R2 x a * R1 a y \<noteq> 0} = {a. R2 x a \<noteq> 0 \<and> R1 a y \<noteq> 0}" by simp
-  also have "\<dots> \<subseteq> fst ` {(a,a)| a. R2 x a \<noteq> 0 \<and> R1 a y \<noteq> 0}" by auto
-  also have "\<dots> \<subseteq> fst ` ({a. R2 x a \<noteq> 0} \<times> {a. R1 a y \<noteq> 0})"
+  have "{a. the_acost (R2 x) a * the_acost (R1 a) y \<noteq> 0} = {a. the_acost (R2 x) a \<noteq> 0 \<and> the_acost (R1 a) y \<noteq> 0}" by simp
+  also have "\<dots> \<subseteq> fst ` {(a,a)| a. the_acost (R2 x) a \<noteq> 0 \<and> the_acost (R1 a) y \<noteq> 0}" by auto
+  also have "\<dots> \<subseteq> fst ` ({a. the_acost (R2 x) a \<noteq> 0} \<times> {a. the_acost (R1 a) y \<noteq> 0})"
     apply(rule image_mono) by auto
   finally
   show ?thesis apply(rule finite_subset)
     apply(rule finite_imageI)
     apply(rule finite_cartesian_product)
-    apply(rule wfR_snd) apply fact
+    apply(rule wfR_snd[where R=R2]) apply fact
     apply(rule wfR_fst) by fact
 qed
 
-
-
 lemma wfR_finite_mult_left:
+  fixes R2 :: "('b \<Rightarrow> ('c, 'd::mult_zero) acost)"
   assumes "wfR R2"
-  shows "finite {a. Mc a * R2 a ac \<noteq> (0::enat)}"
+  shows "finite {a. the_acost Mc a * the_acost (R2 a) ac \<noteq> 0}"
 proof -
 
-  have "{a. Mc a * R2 a ac \<noteq> 0} \<subseteq> {a. R2 a ac \<noteq> 0}"
-    by auto
+  have "{a. the_acost Mc a * the_acost (R2 a) ac \<noteq> 0} \<subseteq> {a. the_acost (R2 a) ac \<noteq> 0}"
+    apply(cases Mc) by (auto simp: zero_acost_def)
   then
   show ?thesis
     apply(rule finite_subset)
@@ -77,10 +88,14 @@ qed
 lemma 
   wfR_finite_crossprod:
   assumes "wfR R2"
-  shows "finite ({a. \<exists>b. Mc a * (R2 a b * R1 b cc) \<noteq> (0::enat)} \<times> {b. \<exists>a. Mc a * (R2 a b * R1 b cc) \<noteq> 0})"
+  shows "finite ({a. \<exists>b. the_acost Mc a * (the_acost (R2 a) b * the_acost (R1 b) cc) \<noteq> 0} \<times> {b. \<exists>a. the_acost Mc a * (the_acost (R2 a) b * the_acost (R1 b) cc) \<noteq> 0})"
 proof -
-  have i: "{a. \<exists>b. Mc a * (R2 a b * R1 b cc) \<noteq> 0} \<subseteq> fst ` ({(a,b).  R2 a b \<noteq> 0} \<inter> {(a,b). R1 b cc \<noteq> 0})" by auto
-  have ii: "{b. \<exists>a. Mc a * (R2 a b * R1 b cc) \<noteq> 0} \<subseteq> snd ` ({(a,b).  R2 a b \<noteq> 0} \<inter> {(a,b). R1 b cc \<noteq> 0})" by auto
+  have i: "{a. \<exists>b. the_acost Mc a * (the_acost (R2 a) b * the_acost (R1 b) cc) \<noteq> 0} \<subseteq> fst ` ({(a,b).  the_acost (R2 a) b \<noteq> 0} \<inter> {(a,b). the_acost (R1 b) cc \<noteq> 0})"
+    apply safe 
+    by (metis (mono_tags, lifting) Int_iff arith_simps(62) arith_simps(63) case_prodI image_eqI mem_Collect_eq prod.sel(1))  
+  have ii: "{b. \<exists>a. the_acost Mc a * (the_acost (R2 a) b * the_acost (R1 b) cc) \<noteq> 0} \<subseteq> snd ` ({(a,b).  the_acost (R2 a) b \<noteq> 0} \<inter> {(a,b). the_acost (R1 b) cc \<noteq> 0})"
+    apply safe  
+    by (metis (mono_tags, lifting) Int_iff arith_simps(62) arith_simps(63) case_prodI image_eqI mem_Collect_eq prod.sel(2))  
   
 
   show ?thesis 
@@ -94,17 +109,17 @@ qed
 
 lemma wfR_finite_Sum_any: 
   assumes *: "wfR R"
-  shows "finite {x. ((Sum_any (\<lambda>ac. ((Mc ac) * (R ac x)))) \<noteq> (0::enat))}"
+  shows "finite {x. ((Sum_any (\<lambda>ac. (the_acost Mc ac * (the_acost (R ac) x)))) \<noteq> 0)}"
 proof - 
   {fix x
-    have "((Sum_any (\<lambda>ac. ((Mc ac) * (R ac x)))) \<noteq> 0)
-      \<Longrightarrow> \<exists>ac. (Mc ac) * (R ac x) \<noteq> 0"
+    have "((Sum_any (\<lambda>ac. ((the_acost Mc ac) * (the_acost (R ac) x)))) \<noteq> 0)
+      \<Longrightarrow> \<exists>ac. (the_acost Mc ac) * (the_acost (R ac) x) \<noteq> 0"
       using Sum_any.not_neutral_obtains_not_neutral by blast 
   } then 
-  have "{x. ((Sum_any (\<lambda>ac. ((Mc ac) * (R ac x)))) \<noteq> 0)}
-          \<subseteq> {x. \<exists>ac. ((Mc ac) * (R ac x)) \<noteq> 0}" by blast
-  also have "\<dots> \<subseteq> snd ` {(ac,x). ((Mc ac) * (R ac x)) \<noteq> 0}" by auto 
-  also have "\<dots> \<subseteq> snd ` {(ac,x).  (R ac x) \<noteq> 0}" by auto
+  have "{x. ((Sum_any (\<lambda>ac. ((the_acost Mc ac) * (the_acost (R ac) x)))) \<noteq> 0)}
+          \<subseteq> {x. \<exists>ac. ((the_acost Mc ac) * (the_acost (R ac) x)) \<noteq> 0}" by blast
+  also have "\<dots> \<subseteq> snd ` {(ac,x). ((the_acost Mc ac) * (the_acost (R ac) x)) \<noteq> 0}" by auto 
+  also have "\<dots> \<subseteq> snd ` {(ac,x).  (the_acost (R ac) x) \<noteq> 0}" by auto
 
   finally  show ?thesis 
     apply(rule finite_subset )
@@ -112,18 +127,19 @@ proof -
 qed 
 
 
-
+(*
 lemma assumes "R' \<le> R" "wfR R" shows "wfR R'"
 proof -                                    
-  from assms(1) have *: "\<And> a b. R' a b\<le> R a b"
-  unfolding le_fun_def   by auto
-  {fix  a b have "R a b  = 0 ==> R' a b = 0 "   
-      using * [of a b] by auto}
+  from assms(1) have *: "\<And> a b. the_acost (R' a) b\<le> the_acost (R a) b"
+  unfolding less_eq_acost_def le_fun_def   by auto
+  {fix  a b have "the_acost (R a) b  = 0 \<Longrightarrow> the_acost (R' a) b = 0 "   
+      using * [of a b] by (auto simp: zero_acost_def less_eq_acost_def)}
   note f=this
   show "wfR R'"
     using \<open>wfR R\<close> unfolding wfR_def apply(rule rev_finite_subset)
     apply safe using f by simp
 qed
+*)
 
 lemma wfn_timerefine: "wfn m \<Longrightarrow> wfR R \<Longrightarrow> wfn (timerefine R m)"
 proof -
@@ -138,39 +154,42 @@ qed
 lemma [simp]: "timerefine R FAILT = FAILT" by(auto simp: timerefine_def)
 
 definition pp where
-  "pp R2 R1 = (\<lambda>a c. Sum_any (%b. R1 a b * R2 b c  ) )"
+  "pp R2 R1 = (\<lambda>a. acostC (\<lambda>c. Sum_any (%b. the_acost (R1 a) b * the_acost (R2 b) c  ) ))"
 
 lemma Sum_any_mono:
-  assumes fg: "\<And>x.    f x \<le> g x"
-    and finG: "finite {x. g x \<noteq> (0::enat)}"
+  fixes f :: "('a \<Rightarrow> 'b::{nonneg,comm_monoid_add,order,ordered_comm_monoid_add})"
+  assumes fg: "\<And>x. f x \<le> g x" (* can one relax that and say the norm is mono, for integer domains ? *)
+    and finG: "finite {x. g x \<noteq> 0}"
 shows "Sum_any f \<le> Sum_any g"
 proof -
-  have "{x. f x \<noteq> (0::enat)} \<subseteq> {x. g x \<noteq> (0::enat)}"
-    apply auto using fg   
-    by (metis ile0_eq)  
-  with finG have "finite {x. f x \<noteq> (0::enat)}"  
+  have "{x. f x \<noteq> 0} \<subseteq> {x. g x \<noteq> 0}"
+    apply auto
+    subgoal for x using fg[of x] needname_nonneg[of " f x"] by auto 
+    done
+  with finG have "finite {x. f x \<noteq> 0}"  
     using finite_subset by blast   
 
   thm sum_mono sum_mono2
-  
-  have "sum f {x. f x \<noteq> (0::enat)} \<le> sum f {x. g x \<noteq> (0::enat)}"
+  thm sum_mono2
+  have "sum f {x. f x \<noteq> 0} \<le> sum f {x. g x \<noteq> 0}"
     apply(rule sum_mono2) apply fact apply fact
     by simp
-  also have "\<dots> \<le> sum g {x. g x \<noteq> (0::enat)}"
+  also have "\<dots> \<le> sum g {x. g x \<noteq> 0}"
     apply(rule sum_mono) using fg by simp
   finally show ?thesis unfolding Sum_any.expand_set .
 qed
 
 lemma finite_support_mult:  
-  assumes "finite {xa.  R1 xa \<noteq> (0::enat)}"
-  and "finite {xa. R2 xa \<noteq> 0}"
-shows "finite {xa. R2 xa * R1 xa \<noteq> 0}"
+  fixes R1 :: "('a, 'b::{semiring_no_zero_divisors}) acost"
+  assumes "finite {xa.  the_acost R1 xa \<noteq> 0}"
+  and "finite {xa. the_acost R2 xa \<noteq> 0}"
+shows "finite {xa. the_acost R2 xa * the_acost R1 xa \<noteq> 0}"
 proof -
  
-  have "{(xa,xa)|xa. R2 xa * R1 xa \<noteq> 0} = {(xa,xa)|xa. R2 xa \<noteq> 0 \<and> R1 xa \<noteq> 0}" by auto
-  also have "\<dots> \<subseteq> {(xa,xb)|xa xb. R2 xa \<noteq> 0 \<and> R1 xb \<noteq> 0}" by auto
-  also have "\<dots> = {xa. R2 xa \<noteq> 0} \<times> {xb. R1 xb \<noteq> 0}" by auto 
-  finally have k: "{xa. R2 xa * R1 xa \<noteq> 0} \<subseteq> fst ` ({xa. R2 xa \<noteq> 0} \<times> {xb. R1 xb \<noteq> 0})" by blast
+  have "{(xa,xa)|xa. the_acost R2 xa * the_acost R1 xa \<noteq> 0} = {(xa,xa)|xa. the_acost R2 xa \<noteq> 0 \<and> the_acost R1 xa \<noteq> 0}" by auto
+  also have "\<dots> \<subseteq> {(xa,xb)|xa xb. the_acost R2 xa \<noteq> 0 \<and> the_acost R1 xb \<noteq> 0}" by auto
+  also have "\<dots> = {xa. the_acost R2 xa \<noteq> 0} \<times> {xb. the_acost R1 xb \<noteq> 0}" by auto 
+  finally have k: "{xa. the_acost R2 xa * the_acost R1 xa \<noteq> 0} \<subseteq> fst ` ({xa. the_acost R2 xa \<noteq> 0} \<times> {xb. the_acost R1 xb \<noteq> 0})" by blast
 
   show ?thesis
     apply(rule finite_subset[OF k])
@@ -180,41 +199,49 @@ qed
 
 
 lemma timerefine_mono: 
+  fixes R :: "_ \<Rightarrow> ('a, 'b::{complete_lattice,nonneg,mult_zero,ordered_semiring}) acost"
   assumes "wfR R"
   shows "c\<le>c' \<Longrightarrow> timerefine R c \<le> timerefine R c'"
   apply(cases c) apply simp
-  apply(cases c') apply (auto simp: timerefine_def split: nrest.splits option.splits simp: le_fun_def)
+  apply(cases c') apply (auto simp: less_eq_acost_def timerefine_def split: nrest.splits option.splits simp: le_fun_def)
   subgoal  by (metis le_some_optE) 
   proof (goal_cases)
     case (1 x2 x2a x x2b x2c xa)
-    then have l: "\<And>ac. x2b ac \<le> x2c ac"  
-      by (metis le_funD less_eq_option_Some)    
-    show ?case 
+    then have l: "\<And>ac. the_acost x2b ac \<le>  the_acost x2c ac"
+      apply(cases x2b; cases x2c) unfolding less_eq_acost_def  
+      apply auto
+      by (metis acost.sel less_eq_acost_def less_eq_option_Some)
+    show ?case
       apply(rule Sum_any_mono)
-      subgoal using l apply(rule mult_right_mono) by simp
+      subgoal using l apply(rule ordered_semiring_class.mult_right_mono) by (simp add: needname_nonneg)
       apply(rule wfR_finite_mult_left) by fact
   qed 
 
 
-lemma assumes "wfR R1" "wfR R2"
+lemma
+  fixes R1 :: "_ \<Rightarrow> ('a, 'b::{complete_lattice,nonneg,ordered_semiring,semiring_no_zero_divisors}) acost"
+  assumes "wfR R1" "wfR R2"
   shows timerefine_iter: "timerefine R1 (timerefine R2 c) =  timerefine (pp R1 R2) c"
   unfolding timerefine_def 
-  apply(cases c) apply simp 
+  apply(cases c)
+  subgoal by simp 
   apply (auto simp: le_fun_def pp_def split: option.splits) apply (rule ext)
-  apply (auto simp: le_fun_def pp_def split: option.splits) 
-    apply(subst Sum_any_right_distrib)
-  subgoal apply(rule finite_wfR_middle_mult) using assms by simp_all
-    apply (rule ext)
+  apply (auto simp: le_fun_def pp_def split: option.splits)
+  apply(subst Sum_any_right_distrib)
+  subgoal apply(rule finite_wfR_middle_mult[of R1 R2]) using assms by simp_all
+  apply (rule ext)
   subgoal for mc r Mc cc
-        apply (subst Sum_any.swap[where C="{a. \<exists>b. Mc a * (R2 a b * R1 b cc) \<noteq> 0} \<times> {b. \<exists>a. Mc a * (R2 a b * R1 b cc) \<noteq> 0}"])
-        subgoal apply(rule wfR_finite_crossprod) using assms by simp
-        subgoal by simp 
-        apply(subst Sum_any_left_distrib)
-        subgoal apply(rule wfR_finite_mult_left) using assms by simp 
-        by (meson Sum_any.cong ab_semigroup_mult_class.mult_ac(1))  
-      done 
+    apply (subst Sum_any.swap[where C="{a. \<exists>b. the_acost Mc a * (the_acost (R2 a) b * the_acost (R1 b) cc) \<noteq> 0} \<times> {b. \<exists>a. the_acost Mc a * (the_acost (R2 a) b * the_acost (R1 b) cc) \<noteq> 0}"])
+    subgoal apply(rule wfR_finite_crossprod) using assms by simp
+    subgoal by simp 
+    apply(subst Sum_any_left_distrib)
+    subgoal apply(rule wfR_finite_mult_left) using assms by simp 
+    apply(rule Sum_any.cong)
+    by (meson mult.assoc)
+  done 
 
 lemma timerefine_trans: 
+  fixes R1 :: "_ \<Rightarrow> ('a, 'b::{complete_lattice,nonneg,ordered_semiring,semiring_no_zero_divisors}) acost"
   assumes "wfR R1" "wfR R2" shows 
   "a \<le> timerefine R1 b \<Longrightarrow> b \<le> timerefine R2 c \<Longrightarrow> a \<le> timerefine (pp R1 R2) c"
   apply(subst timerefine_iter[symmetric, OF assms])
@@ -222,7 +249,22 @@ lemma timerefine_trans:
     apply(rule timerefine_mono) using assms by auto
 
    
+section \<open>enum setup\<close>
 
+ 
+
+lemma (in enum) sum_to_foldr: "sum f UNIV  
+      = foldr (\<lambda>x a. a + f x) enum 0"
+  (*= sum_list (map f enum_class.enum)"  *)
+  unfolding UNIV_enum using enum_distinct
+  apply(simp add: sum.distinct_set_conv_list  )
+  apply(simp only: sum_list.eq_foldr foldr_map)  
+  by (metis add.commute comp_apply)  
+
+lemma (in enum) Sum_any_to_foldr: "Sum_any f  
+      = foldr (\<lambda>x a. a + f x) enum 0"
+  apply(subst Sum_any.expand_superset[where A=UNIV])
+  by (simp_all add: sum_to_foldr)
 
 
 end
